working

MyMain.thy
@@ -1,77 +1,78 @@
 theory MyMain
   imports Main MyOCL MySQL
 begin
-datatype Person = P string
+(* Person(id, age, email) *)
+datatype Person = P string int string
+type_synonym persons = "Person list" 
 
-datatype val = VInt int | VString string 
-  | VBool bool | VPerson Person | VList "val list"
+datatype val =  VInt int | VString string 
+  |  VBool bool |  VPerson Person | VList vlist
+and vlist = VNil | VCons val vlist
 
-datatype pair = Pair col "string \<Rightarrow> int"
+fun proj :: "col \<Rightarrow> Person \<Rightarrow> val" where
+"proj (AGE) (P pid page pemail) = VInt page" |
+"proj (EMAIL) (P pid page pemail) = VString pemail" |
+"proj (ID) (P pid page pemail) = VString pid" 
 
-datatype objectModel = OM "pair list"
-
-fun doNothing :: "string \<Rightarrow> int" where
-"doNothing s = 0"
-
-function findAtt :: "col \<Rightarrow> objectModel \<Rightarrow> (string \<Rightarrow> int)" where
-"findAtt _ (OM Nil) = doNothing" |
-"findAtt col (OM (Cons (Pair col1 f) xs)) = 
-(if equalCol col col1 then f else findAtt col (OM xs))"
-  by pat_completeness auto
-
-fun equalPerson :: "Person \<Rightarrow> Person \<Rightarrow> bool" where
-"equalPerson (P s1) (P s2) = (s1 = s2)"
+fun ext :: "var \<Rightarrow> col \<Rightarrow> persons \<Rightarrow> val" where
+"ext v col Nil = VString ''null''" |
+"ext v col (Cons (P pid page pemail) ps) 
+  = 
+(if (v = pid) then (proj col (P pid page pemail))  
+else (ext v col ps))"
 
 fun equalVal :: "val \<Rightarrow> val \<Rightarrow> bool" where
 "equalVal (VInt i1) (VInt i2) = (i1 = i2)" |
 "equalVal (VBool b1) (VBool b2) = (b1 \<longleftrightarrow> b2)" |
 "equalVal (VString s1) (VString s2) = (s1 = s2)" |
 "equalVal (VPerson p1) (VPerson p2) = (p1 = p2)" |
-"equalVal (VList Nil) (VList Nil) = True" |
-"equalVal (VList (Cons v1 v1s)) (VList (Cons v2 v2s)) = 
+"equalVal (VList VNil) (VList VNil) = True" |
+"equalVal (VList (VCons v1 v1s)) (VList (VCons v2 v2s)) = 
 (if (equalVal v1 v2) then (equalVal (VList v1s) (VList v2s)) else False)" |
 "equalVal _ _ = False" 
 
-function (sequential) exec :: "SQLstm \<Rightarrow> objectModel \<Rightarrow> val" where
-"exec (Select (MySQL.Int i)) om = VInt i" |
-
-"exec (Select (MySQL.Var v)) om = VString v" |
-
-"exec (Select (MySQL.Col _)) om = VString ''null''" |
-
-"exec (Select (MySQL.Eq (MySQL.Var v1) (MySQL.Var v2))) om = 
+function (sequential) exec :: "SQLstm \<Rightarrow> persons \<Rightarrow> val" where
+"exec (Select (MySQL.Int i)) ps  = VInt i" |
+"exec (Select (MySQL.Var v)) ps = VString v" |
+"exec (Select (MySQL.Col _)) ps = VString ''null''" |
+"exec (Select (MySQL.Eq (MySQL.Var v1) (MySQL.Var v2))) ps = 
 VBool (v1 = v2)" |
-
-"exec (Select (MySQL.Eq (MySQL.Int i1) (MySQL.Int i2))) om = 
+"exec (Select (MySQL.Eq (MySQL.Int i1) (MySQL.Int i2))) ps = 
 VBool (i1 = i2)" |
-
-"exec (Select (MySQL.Eq (MySQL.Col c1) (MySQL.Col c2))) om = 
+"exec (Select (MySQL.Eq (MySQL.Col c1) (MySQL.Col c2))) ps = 
 VBool (c1 = c2)" |
-
-"exec (Select (MySQL.Eq _ _)) om = VBool False" |
-
-"exec (SelectFrom _ _) om = VBool False" |
-
+"exec (Select (MySQL.Eq _ _)) ps = VBool False" |
+(* TBC: partial definition *)
+"exec (SelectFrom _ _) ps = VBool False" |
+(* FROM_WHERE *)
 "exec (SelectFromWhere (MySQL.Col col) (FROM table1) 
-(WHERE (MySQL.Eq (MySQL.Col col2) (MySQL.Var v)))) om
-= (if isID col2 table1 then VInt ((findAtt col om) v) else VBool False)" |
+(WHERE (MySQL.Eq (MySQL.Col col2) (MySQL.Var v)))) ps
+= (if isID col2 table1 
+then (ext v col ps) 
+else VBool False)" |
 
 "exec (SelectFromWhere (MySQL.Eq (MySQL.Col col1) (MySQL.Int i)) 
 (FROM table) 
-(WHERE (MySQL.Eq (MySQL.Col col2) (MySQL.Var v)))) om
+(WHERE (MySQL.Eq (MySQL.Col col2) (MySQL.Var v)))) ps
 = VBool (equalVal (exec (SelectFromWhere (MySQL.Col col1) (FROM table) 
-(WHERE (MySQL.Eq (MySQL.Col col2) (MySQL.Var v)))) om) (VInt i))" |
+(WHERE (MySQL.Eq (MySQL.Col col2) (MySQL.Var v)))) ps ) (VInt i))" |
 
-"exec _ om = VBool False"
-
-  by pat_completeness auto
+"exec _ ps = VBool False"
+by pat_completeness auto
 termination by size_change
 
-fun eval :: "OCLexp \<Rightarrow> objectModel \<Rightarrow> val" where
-"eval (MyOCL.Int i) om = VInt i" |
-"eval (MyOCL.Var x) om = VString x" |
-"eval (MyOCL.Eq e1 e2) om = VBool (equalVal (eval e1 om) (eval e2 om))" |
-"eval (MyOCL.Att v col) om = VInt ((findAtt (ATT col) om) v)"
+fun trans :: "MyOCL.att \<Rightarrow> MySQL.col" where
+"trans MyOCL.AGE = MySQL.AGE" |
+"trans MyOCL.EMAIL = MySQL.EMAIL" |
+"trans MyOCL.ID = MySQL.ID" 
+
+fun eval :: "OCLexp \<Rightarrow> persons \<Rightarrow> val" where
+"eval (MyOCL.Int i) ps = VInt i" |
+"eval (MyOCL.Var x) ps = VString x" |
+"eval (MyOCL.Eq e1 e2) ps = 
+VBool (equalVal (eval e1 ps) (eval e2 ps))" |
+"eval (MyOCL.Att v att) ps 
+= ext v (trans att) ps"
 
 (* self = caller *)
 lemma "\<forall> self caller om. eval (MyOCL.Eq (MyOCL.Var self) (MyOCL.Var caller)) om 
@@ -80,10 +81,10 @@ proof auto
 qed
 
 (* self.age = 30 *)
-lemma "\<forall> om self. eval (MyOCL.Eq (MyOCL.Att self age) (MyOCL.Int 30)) om
-= exec (SelectFromWhere (MySQL.Eq (MySQL.Col (ATT age)) (MySQL.Int 30))
+lemma "\<forall> om self. eval (MyOCL.Eq (MyOCL.Att self MyOCL.AGE) (MyOCL.Int 30)) om
+= exec (SelectFromWhere (MySQL.Eq (MySQL.Col (MySQL.AGE)) (MySQL.Int 30))
 (FROM table)
-(WHERE (MySQL.Eq (MySQL.Col (ID table)) (MySQL.Var self)))) om"
+(WHERE (MySQL.Eq (MySQL.Col (MySQL.ID)) (MySQL.Var self)))) om"
 proof auto
 qed
 
