MySQL.thy
@@ -5,38 +5,24 @@ begin
 type_synonym var = string
 
 type_synonym table = string
-datatype col = ATT string | ID table
+datatype col = AGE  | EMAIL | ID
+
 
 datatype exp = Int int 
   | Var var 
   | Eq exp exp
   | Col col
 
-datatype fromItem = FROM table
 
 datatype whereClause = WHERE exp
 
-datatype SQLstm = Select exp
+datatype SQLstm = Select exp 
   | SelectFrom exp fromItem
-  | SelectFromWhere exp fromItem whereClause
+  | SelectFromWhere exp fromItem whereClause 
+and  fromItem = FROM table |  Subselect SQLstm
 
 fun isID :: "col \<Rightarrow> table \<Rightarrow> bool" where
-"isID (ID t1) t = (t1 = t)" |
+"isID (ID) t = True " |
 "isID _ _ = False"
-
-fun equalCol :: "col \<Rightarrow> col \<Rightarrow> bool" where 
-"equalCol (ATT s1) (ATT s2) = (s1 = s2)" |
-"equalCol (ID i1) (ID i2) = (i1 = i2)" |
-"equalCol _ _ = False"
-
-(* SELECT self = caller *)
-value "Select (Eq (Var self) (Var caller))"
-
-(* SELECT age FROM Lecturer *)
-value "SelectFrom (Att age) (FROM Lecturer)"
-
-(* SELECT age = 30 FROM Lecturer WHERE lid = self *)
-value "SelectFromWhere (Eq (Att age) (MySQL.Int 30))
-(FROM Lecturer) (WHERE (Eq (Att lid) (Var self)))"
 
 end
